IsoGraph.lean
@@ -20,3 +20,4 @@ import IsoGraph.Invariants
 import IsoGraph.Constructions
 import IsoGraph.Compute
 import IsoGraph.Enumerate
+import IsoGraph.EnumerateConn
